finished porting the examples.

examples/ExprDemo.v
@@ -6,19 +6,21 @@ Require Import MirrorCore.Ext.Expr.
 (** Demo **)
 Section Demo.
   Definition types' : types.
-  refine ({| Impl := nat ; Eqb := fun _ _ => None |} :: 
+  refine ({| Impl := nat ; Eqb := fun _ _ => None |} ::
           {| Impl := list nat ; Eqb := fun _ _ => None |} :: nil); auto.
   Defined.
 
   Definition all (T : Type) (P : T -> Prop) : Prop :=
     forall x, P x.
 
-  Definition typD := typD types'. 
+  Definition typD := typD types'.
 
-  Definition funcs' : functions typD.
-  refine (F _ 0
-             (tvArr (tvType 0) (tvArr (tvType 0) (tvType 0)))
-             plus :: 
+  Let tvNat := tvType 0.
+
+  Definition funcs' : functions types'.
+  refine (F types' 0
+             (tvArr tvNat (tvArr tvNat tvNat))
+             plus ::
           F _ 1
              (tvArr (tvArr (tvVar 0) tvProp) tvProp) 
              (fun x : Type => @ex x) ::
@@ -28,16 +30,15 @@ Section Demo.
           F _ 1
              (tvArr (tvVar 0) (tvArr (tvVar 0) tvProp))
              (fun T : Type => @eq T) ::
+          F types' 0 (tvType 0) 0 ::
           nil).
   Defined.
 
-  
-
   Goal
-    let e := @App _ _ (@Func _ _ 1 (tvType 0 :: nil))
-                    ((@Abs _ _ (tvType 0) (@App _ _ (@Func _ _ 3 (tvType 0 :: nil))
-                                                ((Var 0) :: @Const _ _ (tvType 0) 0 :: nil))) :: nil) in
-    match @exprD typ typD _ _ _ funcs' nil nil e tvProp with 
+    let e := @App (@Func 1 (tvType 0 :: nil))
+                    ((@Abs tvNat (@App (@Func 3 (tvType 0 :: nil))
+                                                ((Var 0) :: @Func 4 nil :: nil))) :: nil) in
+    match @exprD _ funcs' nil nil e tvProp with
       | None => False
       | Some p => p
     end.
