examples/Monad/MonadDemo.v
@@ -23,10 +23,10 @@ Module demo.
   Context {typ_m : TypInstance1 typD m}.
   Context {typ_nat : TypInstance0 typD nat}.
 
-  Definition mr : mexpr typ -> mexpr typ := 
+  Definition mr : mexpr typ -> mexpr typ :=
     @monad_run m typ typD (mexpr typ) _ typ_arr typ_m
         (@SApp_bind2 m _ typ typD _ typ_arr typ_m typ_nat)
-        (@SApp_ret1 m _ typ typD _ typ_arr typ_m typ_nat) 
+        (@SApp_ret1 m _ typ typD _ typ_arr typ_m typ_nat)
         (@gen_app m _ typ typD _ typ_arr typ_m typ_nat)
         (@Lambda_abs m _ _ typD _ typ_arr typ_m typ_nat).
 
