examples/Monad/MonadReduce.v
@@ -3,8 +3,8 @@ Require Import ExtLib.Structures.Monads.
 Require Import ExtLib.Data.Fun.
 Require Import ExtLib.Data.Vector.
 Require Import ExtLib.Data.Monads.FuelMonad.
-Require Import MirrorCore.TypesExt.
-Require Import MirrorCore.ExprExt.
+Require Import MirrorCore.TypesI.
+Require Import MirrorCore.ExprI.
 
 Set Implicit Arguments.
 Set Strict Implicit.
@@ -19,20 +19,21 @@ Section Demo.
   Variable expr : Type.
   Context {RType_typ : RType typD}.
   Context {RTypeOk_typ : RTypeOk RType_typ}.
+  Context {Expr_expr : Expr typD expr}.
   Context {typ_arr : TypInstance2 typD Fun}.
   Context {typ_m : TypInstance1 typD m}.
   Let tvArr := @typ2 _ typD _ typ_arr.
   Let tvM := @typ1 _ typD _ typ_m.
 
-  Variable bind_app : @SymAppN typ expr 2 ((fun x => tvM (vector_hd x)) :: (fun x => tvArr (vector_hd x) (tvM (vector_hd (vector_tl x)))):: nil) (fun _ => tvM).
-  Variable ret_app : @SymAppN typ expr 1 (vector_hd :: nil) tvM.
-  Variable app_i : forall d r, AppInstance typD expr (tvArr d r) d r.
-  Variable lam : Lambda typ expr.
+  Variable bind_app : @SymAppN typ _ expr _ 2 ((fun x => tvM (vector_hd x)) :: (fun x => tvArr (vector_hd x) (tvM (vector_hd (vector_tl x)))):: nil) (fun _ => tvM).
+  Variable ret_app : @SymAppN typ _ expr _ 1 (vector_hd :: nil) tvM.
+  Variable app_i : forall d r, @AppInstance typ typD expr _ (tvArr d r) d r.
+  Variable lam : @Lambda typ typD expr _.
 
-  Let Bind (t1 t2 : typ) (b1 b2 : expr) : expr := 
+  Let Bind (t1 t2 : typ) (b1 b2 : expr) : expr :=
     sappn bind_app (Vcons t1 (Vcons t2 (Vnil _)))
                    (Vcons b1 (Vcons b2 (Vnil _))).
-  Let Ret (t1 : typ) (b1 : expr) : expr := 
+  Let Ret (t1 : typ) (b1 : expr) : expr :=
     sappn ret_app (Vcons t1 (Vnil _))
                   (Vcons b1 (Vnil _)).
 
@@ -40,9 +41,12 @@ Section Demo.
                                     (caseBind : typ -> typ -> expr -> expr -> R)
                                     (caseElse : unit -> R) (e : expr) : R :=
     match sappn_check bind_app e with
-      | Some (vs,es) => caseBind (vector_hd vs) (vector_hd (vector_tl vs)) (vector_hd es) (vector_hd (vector_tl es))
+      | Some (existT (vs,es) _) =>
+        caseBind (vector_hd vs) (vector_hd (vector_tl vs))
+                 (vector_hd es) (vector_hd (vector_tl es))
       | None => match sappn_check ret_app e with
-                  | Some (vs,es) => caseRet (vector_hd vs) (vector_hd es)
+                  | Some (existT (vs,es) _) =>
+                    caseRet (vector_hd vs) (vector_hd es)
                   | None => caseElse tt
                 end
     end.
@@ -55,11 +59,12 @@ Section Demo.
   Definition monad_run' : expr -> GFix expr.
   refine (
       mfix (fun recur e =>
-              let do_lam e := 
+              let do_lam e :=
                   match lambda_check lam e with
                     | None => ret (inl e)
-                    | Some (t,e) => e' <- recur e ;;
-                                    ret (inr (t,e'))
+                    | Some (existT (t,e) _) =>
+                      e' <- recur e ;;
+                      ret (inr (t,e'))
                   end
               in
       @monad_match (GFix expr)
@@ -67,19 +72,19 @@ Section Demo.
         (fun t1 t2 b1 b2 =>
            b1' <- recur b1 ;;
            match sappn_check ret_app b1' with
-             | None => 
+             | None =>
                b2' <- do_lam b2 ;;
                match b2' with
                  | inl b2' => ret (Bind t1 t2 b1' b2)
                  | inr (t,b2') => ret (Bind t1 t2 b1' (lambda lam t b2'))
                end
-             | Some (t, v) =>
+             | Some (existT (t, v) _) =>
                let t := vector_hd t in
                let v := vector_hd v in
                b2' <- do_lam b2 ;;
                match b2' with
-                 | inl b2' => 
-                   ret (@app1 _ typD expr _ _ _ (app_i t (tvM t2)) b2' v)
+                 | inl b2' =>
+                   ret (@app1 _ typD expr _ _ _ _ (app_i t (tvM t2)) b2' v)
                  | inr (_, b2') =>
                    let b2' := subst0 lam b2' v in
                    recur b2'
@@ -94,5 +99,5 @@ Section Demo.
       | Term e => e
       | Diverge => e
     end.
-    
+
 End Demo.
